added Opaque type syntax

rustexamples/test/borrow_test/40.rs
@@ -1,0 +1,5 @@
+fn main(){
+    let b: Box<i32> = Box(1);
+    let p: &mut Box<i32> = &mut b; // FIXME: memory leak here because we do not generate drop(*p) for now. But I think leaking is not UB.
+    *p = Box(2);
+}
