rustfrontend/RustOp.v
@@ -406,6 +406,11 @@ Proof.
     exists (Vptr b2 (Ptrofs.add ofs1 (Ptrofs.repr delta))).
     destruct (ident_eq i 1). split. auto.  
     TrivialInject. eapply Val.inject_ptr; eauto. inv H2. 
+  - destruct t2; inv H0; simpl in *;
+     try (destruct i; simpl in *);
+          try (destruct f0; simpl in *);
+               try (destruct i0; simpl in *);
+               TrivialInject.
   Qed. 
 
 
